SimAsm/SimAsm_StateStack.thy
@@ -41,9 +41,9 @@ print_quot_maps
   
 type_synonym ('var,'val,'a) stack = "('var, 'val,'a) frame_scheme list" 
 
-definition emptyFrame :: "('var,'val) frame" where
-  "emptyFrame \<equiv> \<lparr> frame_st = (\<lambda>v. None),
-                  frame_cap = {} \<rparr>"            (* is cap = emptySet ? *)
+definition emptyFrame :: "'var set \<Rightarrow> ('var,'val) frame" where
+  "emptyFrame cap \<equiv> \<lparr> frame_st = (\<lambda>v. None),
+                  frame_cap = cap \<rparr>"            (* is cap = emptySet ? *)
 
 definition Is_tstack :: "('var,'val,'a) stack \<Rightarrow> bool" where 
   "Is_tstack t \<equiv> t \<noteq> [] \<and> frame_cap (last t) = UNIV \<and> (\<forall>v. frame_st (last t) v \<noteq> None)"
